\textbf{\underline{OZ 1 - Herhaling - Oefening 1:}}
\vspace{0.5cm}

Bereken de volgende \textbf{vectorproducten}:

\begin{enumerate}[(a)]
    \item 
        $ \hat{j} \times \hat{i} $  
    
          \hspace{0.5cm} $ = -(\hat{i} \times \hat{j}) $

          \hspace{0.5cm} $ = -\hat{k} $
    
    \item $ \left( \hat{j} \times \hat{k} \right) \times \hat{j} $
    
          \hspace{0.5cm} $ = \left( \left( 0, 1, 0 \right) \times \left( 0, 0, 1 \right) \right) \times \hat{j} $
    
          \hspace{0.5cm} $ = \left( 1, 0, 0 \right) \times \hat{j} $
    
          \hspace{0.5cm} $ = \hat{i} \times \hat{j} $
    
          \hspace{0.5cm} $ = \hat{k} $
    
    \item $ \hat{j} \times \left( \hat{j} \times \hat{k} \right) $
    
          \hspace{0.5cm} $ = \hat{j} \times \hat{i} $
    
          \hspace{0.5cm} $ = -(\hat{i} \times \hat{j})$
    
          \hspace{0.5cm} $ = -\hat{k} $
    
    \item $ (\hat{j} \times \hat{k}) \cdot (\hat{k} \times (\hat{k} \times \hat{i}) + (\hat{j} \times \hat{k}) \times \hat{j})) $

          \hspace{0.5cm} $ = \hat{i} \cdot (\hat{k} \times \hat{j} + \hat{i} \times \hat{j}) $

          \hspace{0.5cm} $ = \hat{i} \cdot ((-\hat{i}) + \hat{k}) $

          \hspace{0.5cm} $ = (1,0,0) \cdot (-1,0,1) $

          \hspace{0.5cm} $ = -1 $
\end{enumerate}

\vspace{1cm}